src/3d/Options.fsti
@@ -61,3 +61,5 @@ val get_add_include : unit -> ML (list string)
 val make_includes : unit -> ML string
 
 val config_module_name : unit -> ML (option string)
+
+val get_emit_smt_encoding: unit -> ML bool
