src/3d/Z3TestGen.fst
@@ -2,6 +2,10 @@ module Z3TestGen
 module Printf = FStar.Printf
 open FStar.All
 
+module A = Ast
+module T = Target
+module I = InterpreterTarget
+
 let prelude : string =
 "
 (declare-datatypes (T1 T2) ((Pair (mk-pair (first T1) (second T2)))))
@@ -17,10 +21,140 @@ let prelude : string =
   )
 )
 
-(define-fun parse-fail ((x (Seq Int))) (Seq Int)
+(define-fun parse-false ((x (Seq Int))) (Seq Int)
   (as seq.empty (Seq Int))
 )
 "
+
+let mk_constant = function
+  | A.Unit -> "0"
+  | A.Int _ x -> string_of_int x
+  | A.XInt _ x -> x
+  | A.Bool true -> "true"
+  | A.Bool false -> "false"
+
+let mk_app fn = function
+  | None -> fn
+  | Some args -> Printf.sprintf "(%s %s)" fn args
+
+let assert_some = function
+  | None -> failwith "assert_some"
+  | Some x -> x
+
+let mk_op : T.op -> option string -> ML string = function
+  | T.Eq -> mk_app "="
+  | T.Neq -> (fun s -> mk_app "not" (Some (mk_app "=" s)))
+  | T.And -> mk_app "and"
+  | T.Or -> mk_app "or"
+  | T.Not -> mk_app "not"
+  | T.Plus _ -> mk_app "+"
+  | T.Minus _ -> mk_app "-"
+  | T.Mul _ -> mk_app "*"
+  | T.Division _ -> mk_app "/"
+  | T.Remainder _ -> mk_app "%"
+  | T.LT _ -> mk_app "<"
+  | T.GT _ -> mk_app ">"
+  | T.LE _ -> mk_app "<="
+  | T.GE _ -> mk_app ">="
+  | T.IfThenElse -> mk_app "if"
+  | T.Cast _ _ -> assert_some (* casts allowed only if they are proven not to lose precision *)
+  | T.Ext s -> mk_app s
+  | _ -> fun _ -> failwith "mk_op: not supported"
+
+let ident_to_string = A.ident_to_string
+
+let rec mk_expr (e: T.expr) : ML string = match fst e with
+  | T.Constant c -> mk_constant c
+  | T.Identifier i -> ident_to_string i
+  | T.App hd args -> mk_op hd (mk_args args)
+  | _ -> failwith "mk_expr: not supported"
+
+and mk_args_aux accu : (list T.expr -> ML string) = function
+  | [] -> accu
+  | a :: q -> mk_args_aux (Printf.sprintf "%s %s" accu (mk_expr a)) q
+
+and mk_args (l: list T.expr) : ML (option string) = match l with
+  | [] -> None
+  | a :: q -> Some (mk_args_aux (mk_expr a) q)
+
+type reading = { call: string }
+type not_reading = { call: string }
+
+type binders = {
+  is_empty: bool;
+  bind: string;
+  args: string;
+}
+
+let empty_binders : binders = {
+  is_empty = true;
+  bind = "";
+  args = "";
+}
+
+let push_binder (name: string) (typ: string) (b: binders) : binders = {
+  is_empty = false;
+  bind = Printf.sprintf "(%s %s) %s" name typ b.bind;
+  args = Printf.sprintf " %s%s" name b.args;
+}
+
+let mk_function_call (name: string) (b: binders) =
+  Printf.sprintf "%s%s" name b.args
+
+type parser (a: Type) =
+  (* name *) string ->
+  (* binders *) binders ->
+  (* is_toplevel *) bool ->
+  (* out *) (string -> ML unit) ->
+  ML a
+
+let unsupported_parser (a: Type) : Tot (parser a) =
+  fun _ _ _ _ -> failwith "unsupported parser"
+
+let parse_u8 : parser reading =
+  fun _ _ _ _ -> { call = "parse-u8" }
+
+let parse_itype = function
+  | I.UInt8 | I.UInt8BE -> parse_u8
+  | _ -> unsupported_parser _
+
+let parse_app
+  (hd: A.ident)
+  (args: list I.expr)
+: Tot (parser reading)
+= fun _ _ _ _ -> { call = mk_app (ident_to_string hd) (mk_args args) }
+
+let parse_dtyp
+  (d: I.dtyp)
+: Tot (parser reading)
+= match d with
+  | I.DT_IType i -> parse_itype i
+  | I.DT_App hd args -> parse_app hd args
+
+let mk_toplevel_parser
+  (name: string)
+  (binders: string)
+  (body: string)
+: string
+= let input = Printf.sprintf "%s-input" name in
+"(define-fun "^name^" ("^binders^"("^input^" (Seq Int))) (Seq Int)
+   ("^body^" "^input^")
+ )
+"
+
+let maybe_toplevel_parser (p: parser not_reading) : parser not_reading =
+  fun name binders is_toplevel out ->
+    if is_toplevel
+    then begin
+      let name' = Printf.sprintf "%s-body" name in
+      let body = p name' binders false out in
+      out (mk_toplevel_parser name binders.bind body.call);
+      { call = mk_function_call name binders }
+    end
+    else p name binders false out
+
+let parse_false : parser not_reading =
+  maybe_toplevel_parser (fun _ _ _ _ -> { call = "parse-false" })
 
 let mk_wrap_parser
   (name: string)
@@ -29,24 +163,117 @@ let mk_wrap_parser
 : string
 = let input = Printf.sprintf "%s-input" name in
   let tmp = Printf.sprintf "%s-tmp" name in
-  Printf.sprintf
-"(define-fun %s (%s(%s (Seq Int))) (Seq Int)
-   (let ((%s (%s %s)))
-     (if (= (seq.len %s) 0)
+"(define-fun "^name^" ("^binders^"("^input^" (Seq Int))) (Seq Int)
+   (let (("^tmp^" ("^body^" "^input^")))
+     (if (= (seq.len "^tmp^") 0)
        (as seq.empty (Seq Int))
-       (seq.unit (second (seq.nth %s 0)))
+       (seq.unit (second (seq.nth "^tmp^" 0)))
      )
    )
  )
 "
-  name
-  binders
-  input
-  tmp
-  body
-  input
-  tmp
-  tmp
+
+let wrap_parser (p: parser reading) : parser not_reading =
+  fun name binders _ out ->
+    let name' = Printf.sprintf "%s-wrapped" name in
+    let body = p name' binders false out in
+    out (mk_wrap_parser name binders.bind body.call);
+    { call = mk_function_call name binders }
+
+let parse_denoted (d: I.dtyp) : parser not_reading =
+  wrap_parser (parse_dtyp d)
+
+let mk_parse_pair
+  (name: string)
+  (binders: string)
+  (fst: string)
+  (snd: string)
+: string
+= let input = Printf.sprintf "%s-input" name in
+  let tmp_has_fst = Printf.sprintf "%s-tmp-has-fst" name in
+  let tmp_fst = Printf.sprintf "%s-tmp-fst" name in
+  let tmp_snd_result = Printf.sprintf "%s-tmp-snd-result" name in
+"(define-fun "^name^" ("^binders^input^" (Seq Int))) (Seq Int)
+   (let (("^tmp_has_fst^" ("^fst^" "^input^")))
+     (if (= (seq.len "^tmp_has_fst^") 0)
+       (as seq.empty (Seq Int))
+       (let (("^tmp_fst^" (seq.nth "^tmp_has_fst^" 0)))
+         (let (("^tmp_snd_result^" ("^snd^" (seq.extract "^input^" "^tmp_fst^" (- (seq.len "^input^") "^tmp_fst^")))))
+             (if (= (seq.len "^tmp_snd_result^") 0)
+               (as seq.empty (Seq Int))
+               (seq.unit (+ "^tmp_fst^" (seq.nth "^tmp_snd_result^" 0)))
+             )
+           )
+         )
+       )
+     )
+   )
+ )"
+
+let parse_pair (fst: parser not_reading) (snd: parser not_reading) : parser not_reading =
+  fun name binders _ out ->
+    let name_fst = Printf.sprintf "%s-fst" name in
+    let body_fst = fst name_fst binders false out in
+    let name_snd = Printf.sprintf "%s-snd" name in
+    let body_snd = snd name_snd binders false out in
+    out (mk_parse_pair name binders.bind body_fst.call body_snd.call);
+    { call = mk_function_call name binders }
+
+let mk_parse_dep_pair_with_refinement
+  (name: string)
+  (binders: string)
+  (dfst: string)
+  (cond_binder_name: string)
+  (cond: string)
+  (dsnd_binder_name: string)
+  (dsnd: string) (* already contains the new argument *)
+: string
+= let input = Printf.sprintf "%s-input" name in
+  let tmp_has_tag = Printf.sprintf "%s-tmp-has-tag" name in
+  let tmp_tag_result = Printf.sprintf "%s-tmp-tag-result" name in
+  let tmp_payload = Printf.sprintf "%s-tmp-payload" name in
+"(define-fun "^name^" ("^binders^"("^input^" (Seq Int))) (Seq Int)
+   (let (("^tmp_has_tag^" ("^dfst^" "^input^")))
+     (if (= (seq.len "^tmp_has_tag^") 0)
+       (as seq.empty (Seq Int))
+       (let (("^tmp_tag_result^" (seq.nth "^tmp_has_tag^" 0)))
+         (if (let (("^cond_binder_name^" (first "^tmp_tag_result^"))) "^cond^")
+           (let (("^dsnd_binder_name^" (first "^tmp_tag_result^")))
+             (let (("^tmp_payload^" ("^dsnd^" (seq.extract "^input^" (second "^tmp_tag_result^") (- (seq.len "^input^") (second "^tmp_tag_result^"))))))
+               (if (= (seq.len "^tmp_payload^") 0)
+                 (as seq.empty (Seq Int))
+                 (seq.unit (+ (second "^tmp_tag_result^") (seq.nth "^tmp_payload^" 0)))
+               )
+             )
+           )
+           (as seq.empty (Seq Int))
+         )
+       )
+     )
+   )
+ )"
+
+let parse_dep_pair_with_refinement_gen (tag: parser reading) (cond_binder: string) (cond: unit -> ML string) (payload_binder: string) (payload: parser not_reading) : parser not_reading =
+  fun name binders _ out ->
+    let name_tag = Printf.sprintf "%s-tag" name in
+    let body_tag = tag name_tag binders false out in
+    let binders' = push_binder payload_binder "Int" binders in (* TODO: support more types *)
+    let name_payload = Printf.sprintf "%s-payload" name in
+    let body_payload = payload name_payload binders' false out in
+    out (mk_parse_dep_pair_with_refinement name binders.bind body_tag.call cond_binder (cond ()) payload_binder body_payload.call);
+    { call = mk_function_call name binders }
+
+let parse_dep_pair_with_refinement (tag: parser reading) (cond_binder: A.ident) (cond: unit -> ML string) (payload_binder: A.ident) (payload: parser not_reading) : parser not_reading =
+  parse_dep_pair_with_refinement_gen tag (ident_to_string cond_binder) cond (ident_to_string payload_binder) payload
+
+let parse_dep_pair (tag: parser reading) (new_binder: A.ident) (payload: parser not_reading) : parser not_reading =
+  parse_dep_pair_with_refinement tag new_binder (fun _ -> "true") new_binder payload
+
+let parse_empty : parser reading =
+  fun _ _ _ _ -> { call = "parse-empty" }
+
+let parse_refine (tag: parser reading) (cond_binder: A.ident) (cond: unit -> ML string) : parser not_reading =
+  parse_dep_pair_with_refinement tag cond_binder cond cond_binder (wrap_parser parse_empty)
 
 let mk_parse_ifthenelse
   (name: string)
@@ -56,134 +283,87 @@ let mk_parse_ifthenelse
   (f_else: string)
 : string
 = let input = Printf.sprintf "%s-input" name in
-  Printf.sprintf
-"(define-fun %s (%s(%s (Seq Int))) (Seq Int)
-   (if %s
-     (%s %s)
-     (%s %s)
+"(define-fun "^name^" ("^binders^"("^input^" (Seq Int))) (Seq Int)
+   (if "^cond^"
+     ("^f_then^" "^input^")
+     ("^f_else^" "^input^")
    )
  )
 "
-  name
-  binders
-  input
-  cond
-  f_then
-  input
-  f_else
-  input
 
-let mk_parse_dtuple2
+let parse_ifthenelse (cond: unit -> ML string) (pthen: parser not_reading) (pelse: parser not_reading) : parser not_reading =
+  fun name binders _ out ->
+    let name_then = Printf.sprintf "%s-then" name in
+    let body_then = pthen name_then binders false out in
+    let name_else = Printf.sprintf "%s-else" name in
+    let body_else = pelse name_else binders false out in
+    out (mk_parse_ifthenelse name binders.bind (cond ()) body_then.call body_else.call);
+    { call = mk_function_call name binders }
+
+let rec parse_typ : I.typ -> parser not_reading = function
+  | I.T_false _ -> parse_false
+  | I.T_denoted _ d
+  | I.T_with_dep_action _ d _ -> wrap_parser (parse_dtyp d)
+  | I.T_pair _ t1 t2 -> parse_pair (parse_typ t1) (parse_typ t2)
+  | I.T_dep_pair _ t1 (lam, t2)
+  | I.T_dep_pair_with_action _ t1 (lam, t2) _ -> parse_dep_pair (parse_dtyp t1) lam (parse_typ t2)
+  | I.T_refine _ base (lam, cond)
+  | I.T_refine_with_action _ base (lam, cond) _ -> parse_refine (parse_dtyp base) lam (fun _ -> mk_expr cond)
+  | I.T_dep_pair_with_refinement _ base (lam_cond, cond) (lam_k, k)
+  | I.T_dep_pair_with_refinement_and_action _ base (lam_cond, cond) (lam_k, k) _ -> parse_dep_pair_with_refinement (parse_dtyp base) lam_cond (fun _ -> mk_expr cond) lam_k (parse_typ k)
+  | I.T_if_else cond t1 t2 -> parse_ifthenelse (fun _ -> mk_expr cond) (parse_typ t1) (parse_typ t2)
+  | I.T_with_action _ base _
+  | I.T_with_comment _ base _ -> parse_typ base
+  | _ -> unsupported_parser _
+
+let smt_type_of_typ (t: T.typ) : Tot string =
+  "Int" (* TODO: support more cases, such as booleans *)
+
+let rec binders_of_params = function
+| [] -> empty_binders
+| (id, t) :: q -> push_binder (ident_to_string id) (smt_type_of_typ t) (binders_of_params q)
+
+let mk_definition
   (name: string)
   (binders: string)
-  (dfst: string)
-  (new_binder_name: string)
-  (dsnd: string) (* already contains the new argument *)
-: string
-= let input = Printf.sprintf "%s-input" name in
-  let tmp_has_tag = Printf.sprintf "%s-tmp-has-tag" name in
-  let tmp_tag_result = Printf.sprintf "%s-tmp-tag-result" name in
-  let tmp_payload = Printf.sprintf "%s-tmp-payload" name in
-  Printf.sprintf
-"(define-fun %s (%s(%s (Seq Int))) (Seq Int)
-   (let ((%s (%s %s)))
-     (if (= (seq.len %s) 0)
-       (as seq.empty (Seq Int))
-       (let ((%s (seq.nth %s 0)))
-         (let ((%s (first %s)))
-           (let ((%s (%s (seq.extract %s (second %s) (- (seq.len %s) (second %s))))))
-             (if (= (seq.len %s) 0)
-               (as seq.empty (Seq Int))
-               (seq.unit (+ (second %s) (seq.nth %s 0)))
-             )
-           )
-         )
-       )
-     )
-   )
- )"
-  name
-  binders
-  input
-  tmp_has_tag
-  dfst
-  input
-  tmp_has_tag
-  tmp_tag_result
-  tmp_has_tag
-  new_binder_name
-  tmp_tag_result
-  tmp_payload
-  dsnd
-  input
-  tmp_tag_result
-  input
-  tmp_tag_result
-  tmp_payload
-  tmp_tag_result
-  tmp_payload
+  (typ: string)
+  (body: string)
+: Tot string
+= "(define-fun "^name^" ("^binders^") "^typ^" "^body^")"
 
-type binders = {
-  bind: string;
-  args: string;
-}
+let produce_definition
+  (i: A.ident)
+  (param: list T.param)
+  (typ: T.typ)
+  (body: T.expr)
+  (out: string -> ML unit)
+: ML unit
+= let binders = binders_of_params param in
+  out (mk_definition (ident_to_string i) binders.bind (smt_type_of_typ typ) (mk_expr body))
 
-let empty_binders : binders = {
-  bind = "";
-  args = "";
-}
+let produce_not_type_decl (a: I.not_type_decl) (out: string -> ML unit) : ML unit =
+  match fst a with
+  | T.Definition (i, param, typ, body) ->
+    produce_definition i param typ body out
+  | T.Assumption _ -> failwith "produce_not_type_decl: unsupported"
+  | T.Output_type _
+  | T.Output_type_expr _ _
+  | T.Extern_type _
+  | T.Extern_fn _ _ _
+  -> ()
 
-let push_binder (name: string) (typ: string) (b: binders) : binders = {
-  bind = Printf.sprintf "(%s %s) %s" name typ b.bind;
-  args = Printf.sprintf " %s%s" name b.args;
-}
+let produce_type_decl (a: I.type_decl) (out: string -> ML unit) : ML unit =
+  let binders = binders_of_params a.name.td_params in
+  let _ = parse_typ a.typ (ident_to_string a.name.td_name) binders true out in
+  ()
 
-let mk_function_call (name: string) (b: binders) =
-  Printf.sprintf "%s%s" name b.args
+let produce_decl (a: I.decl) : (out: string -> ML unit) -> ML unit =
+  match a with
+  | Inl a -> produce_not_type_decl a
+  | Inr a -> produce_type_decl a
 
-type reading = { call: string }
-type not_reading = { call: string }
-
-type parser (a: Type) =
-  (* name *) string ->
-  (* binders *) binders ->
-  (* out *) (string -> ML unit) ->
-  ML a
-
-let parse_u8 : parser reading =
-  fun _ _ _ -> { call = "parse-u8" }
-
-let parse_empty : parser reading =
-  fun _ _ _ -> { call = "parse-empty" }
-
-let parse_fail : parser not_reading =
-  fun _ _ _ -> { call = "parse-fail" }
-
-let wrap_parser (p: parser reading) : parser not_reading =
-  fun name binders out ->
-    let name' = Printf.sprintf "%s-wrapped" name in
-    let body = p name' binders out in
-    out (mk_wrap_parser name binders.bind body.call);
-    { call = mk_function_call name binders }
-
-let parse_ifthenelse (cond: string) (pthen: parser not_reading) (pelse: parser not_reading) =
-  fun name binders out ->
-    let name_then = Printf.sprintf "%s-then" name in
-    let body_then = pthen name_then binders out in
-    let name_else = Printf.sprintf "%s-else" name in
-    let body_else = pelse name_else binders out in
-    out (mk_parse_ifthenelse name binders.bind cond body_then.call body_else.call);
-    { call = mk_function_call name binders }
-
-let parse_dtuple2 (tag: parser reading) (new_binder: string) (payload: parser not_reading) : parser not_reading =
-  fun name binders out ->
-    let name_tag = Printf.sprintf "%s-tag" name in
-    let body_tag = tag name_tag binders out in
-    let binders' = push_binder new_binder "Int" binders in (* TODO: support more types *)
-    let name_payload = Printf.sprintf "%s-payload" name in
-    let body_payload = payload name_payload binders' out in
-    out (mk_parse_dtuple2 name binders.bind body_tag.call new_binder body_payload.call);
-    { call = mk_function_call name binders }
+let produce_decls (l: list I.decl) (out: string -> ML unit) : ML unit =
+  List.iter (fun a -> produce_decl a out) l
 
 let interlude =
 "
@@ -198,6 +378,31 @@ let interlude =
 ))
 "
 
+let produce_prog (l: list I.decl) (out: string -> ML unit) : ML unit =
+  out prelude;
+  produce_decls l out;
+  out interlude
+
+(* Produce the SMT2 encoding of the parser spec *)
+
+let print_prog (l: list I.decl) =
+  produce_prog l FStar.IO.print_string
+
+let with_out_file
+  (#a: Type)
+  (name: string)
+  (body: ((string -> ML unit) -> ML a))
+: ML a
+= let fd = FStar.IO.open_write_file name in
+  let res = body (FStar.IO.write_string fd) in
+  FStar.IO.close_write_file fd;
+  res
+
+let write_prog_to_file (filename: string) (l: list I.decl) : ML unit =
+  with_out_file filename (produce_prog l)
+
+(* Ask Z3 for test witnesses *)
+
 let mk_get_first_witness (name1: string) (name2: string) : string =
   Printf.sprintf
 "
@@ -207,7 +412,6 @@ let mk_get_first_witness (name1: string) (name2: string) : string =
 "
   name1
   name2
-
 
 let read_witness (z3: Z3.z3) =
   Lisp.read_witness_from z3.from_z3
@@ -243,8 +447,8 @@ let witnesses_for (z3: Z3.z3) name1 name2 extra =
 let diff_test (p1: parser not_reading) name1 (p2: parser not_reading) name2 extra =
   let buf : ref string = alloc "" in
   let out x : ML unit = buf := Printf.sprintf "%s%s" !buf x in
-  let name1 = (p1 name1 empty_binders out).call in
-  let name2 = (p2 name2 empty_binders out).call in
+  let name1 = (p1 name1 empty_binders false out).call in
+  let name2 = (p2 name2 empty_binders false out).call in
   Z3.with_z3 (fun z3 ->
     z3.to_z3 prelude;
     z3.to_z3 !buf;
@@ -252,9 +456,3 @@ let diff_test (p1: parser not_reading) name1 (p2: parser not_reading) name2 extr
     witnesses_for z3 name1 name2 extra;
     witnesses_for z3 name2 name1 extra
   )
-
-(*
-let _ =
-  let test1 = parse_dtuple2 parse_u8 "x" (parse_ifthenelse "(< x 12)" parse_fail (parse_dtuple2 parse_u8 "y" (parse_ifthenelse "(> (+ x y) 28)" parse_fail (wrap_parser parse_empty)))) in
-  let test2 = parse_dtuple2 parse_u8 "x" (parse_ifthenelse "(< x 10)" parse_fail (parse_dtuple2 parse_u8 "y" (parse_ifthenelse "(> (+ x y) 30)" parse_fail (wrap_parser parse_u8)))) in
-  diff_test test1 "test1" test2 "test2" 5
